Add files via upload

train.py
@@ -1,0 +1,19 @@
+from openai import OpenAI
+from subprocess import call
+client = OpenAI()
+
+completion = client.chat.completions.create(
+  model="gpt-3.5-turbo",
+  messages=[
+    {"role": "system", "content": "Translate Gallina program to C program. Only include the C program in the content. No need to include a main function in the translated C program, and other English description"},
+    {"role": "user", "content": "Convert Definition swapnum (a b : Z) := (b, a) to C with a and b as pointers. Output the C program only, and not any English with it"}
+  ]
+)
+#print(completion)
+cprog = completion.choices[0].message.content
+#cprog = "void swapnum(int* a, int* b) {  int temp = *a; *a = *b; *b = temp;}"
+fcprog = open("swapprog.c","w")
+fcprog.write(cprog)
+fcprog.close()
+#call clightgen
+call(["clightgen", "-normalize","swapprog.c"])
