Verif_swapsynth.v
@@ -1,12 +1,18 @@
 Require VC.Preface.  (* Check for the right version of VST *)
 Require Import VST.floyd.proofauto.
-Require Import LLMSynth.swap.
+Require Import VC.swap.
 Require Import VST.floyd.local2ptree_denote.
 Require Import VST.floyd.local2ptree_eval.
 Import compcert.lib.Maps.
 
+
 #[export] Instance CompSpecs : compspecs. make_compspecs prog. Defined.
 Definition Vprog : varspecs.  mk_varspecs prog. Defined. (*Global variable*)
+ 
+Check Ebinop.
+Check Omul.
+Check binary_operation.
+Print binary_operation.
 
 (*swap specification*)
 Definition swap_spec : ident * funspec :=
@@ -38,14 +44,14 @@ Definition swapskip_spec : ident * funspec :=
     (*SEP(emp)*)
     SEP (data_at sh1 tint (Vint (Int.repr a)) x; data_at sh2 tint (Vint (Int.repr b)) y).
 
-  Search Int.repr.
+ 
 
 (*math - x is assigned to y + 1*)
 Definition swapmath_spec : ident * funspec :=
   DECLARE _swapmath
    WITH x: val, y: val, sh1 : share, sh2 : share, a : Z, b : Z
    PRE [ tptr tint, tptr tint ]
-    PROP  (readable_share sh1; writable_share sh2;
+    PROP  (readable_share sh1; writable_share sh2; 
     Int.min_signed <= Int.signed (Int.repr a) + Int.signed (Int.repr 1) <= Int.max_signed)
     (*LOCAL (temp _x x; temp _y y)*)
     PARAMS (x; y)
@@ -54,41 +60,43 @@ Definition swapmath_spec : ident * funspec :=
    POST [ tvoid ]
     PROP () RETURN ()
     (*SEP(emp)*)
-    SEP (data_at sh1 tint (Vint (Int.repr a)) x; data_at sh2 tint (Vint (Int.repr (a + 1))) y).
+    SEP (data_at sh1 tint (Vint (Int.repr a)) x; data_at sh2 tint (Vint (Int.repr (a + 1))) y). 
 
 (*if spec: *)
 Definition swapif_spec : ident * funspec :=
   DECLARE _swapif
    WITH x: val, y: val, sh1 : share, sh2 : share, a : Z, b : Z
    PRE [ tptr tint, tptr tint ]
-    PROP  (writable_share sh1; writable_share sh2;
+    PROP  (writable_share sh1; writable_share sh2; 
     Int.min_signed <= a <= Int.max_signed; Int.min_signed <= b <= Int.max_signed)
     (*LOCAL (temp _x x; temp _y y)*)
     PARAMS (x; y)
     (*SEP(emp)*)
     SEP (data_at sh1 tint (Vint (Int.repr a)) x; data_at sh2 tint (Vint (Int.repr b)) y)
    POST [ tvoid ]
-    PROP () RETURN ()
+    PROP () RETURN () 
     (SEPx(
-      if Z_lt_ge_dec a b then
-      (data_at sh1 tint (Vint (Int.repr b)) x :: (data_at sh2 tint (Vint (Int.repr a)) y :: nil))
-      else
+      if Z_lt_ge_dec a b then 
+      (data_at sh1 tint (Vint (Int.repr b)) x :: (data_at sh2 tint (Vint (Int.repr a)) y :: nil)) 
+      else 
       (data_at sh1 tint (Vint (Int.repr b)) x :: (data_at sh2 tint (Vint (Int.repr b)) y :: nil))
       )
     ).
+    
+    
 
 Definition Gprog := [swapskip_spec; swap_spec; swapmath_spec; swapif_spec].
 
 Lemma swapifSynth: semax_body Vprog Gprog f_swapif swapif_spec.
 Proof.
-  start_function. fastforward.
+  start_function. fastforward. 
   destruct (Z_lt_ge_dec a b) eqn:Hzlt. entailer!.
-  contradiction.
+  contradiction. 
   destruct (Z_lt_ge_dec a b) eqn:Hzlt. contradiction. entailer!.
 Qed.
 
 (*auxiliary start function 1: the function specific lemmas are commented out*)
-Ltac start_aux1 :=
+Ltac start_aux1 := 
   (*leaf_function;*)
   lazymatch goal with
   | |- semax_body ?V ?G ?F ?spec =>
@@ -109,7 +117,7 @@ Ltac start_aux1 :=
            | s:=(_, WITH _ : globals PRE [ ] main_pre _ _ _ POST [tint] _):_
              |- _ => idtac
            | s:=?spec':_ |- _ => check_canonical_funspec spec'
-           end; change (semax_body V G F s); subst s;
+           end; change (semax_body V G F s); subst s; 
            unfold NDmk_funspec'
   end;
   let DependedTypeList := fresh "DependedTypeList" in
@@ -132,7 +140,7 @@ Ltac start_aux1 :=
      match goal with
      | |- semax _ (fun rho => (?A rho * ?B rho)%logic) _ _ =>
            change (fun rho => (?A rho * ?B rho)%logic) with (A * B)%logic
-     end;
+     end; 
     simpl functors.MixVariantFunctor._functor in *;
     simpl rmaps.dependent_type_functor_rec; clear DependedTypeList;
     rewrite_old_main_pre;
@@ -145,11 +153,11 @@ Ltac start_aux1 :=
        semax _
          (close_precondition _ match ?p with
                                | (a, b) => _
-                               end * _)%logic _ _ =>
+                               end * _)%logic _ _ => 
        destruct p as [a b]
      | |- semax _ (match ?p with
                    | (a, b) => _
-                   end eq_refl * _)%logic _ _ =>
+                   end eq_refl * _)%logic _ _ => 
        destruct p as [a b]
      | |-
        semax _
@@ -243,7 +251,7 @@ Ltac start_aux3 :=
                | |- _ => intro
                end);
   abbreviate_semaxaux;
-  lazymatch goal with
+  lazymatch goal with 
   | |- semax ?Delta (PROPx _ (LOCALx ?L _)) _ _ => check_parameter_vals Delta L
   | _ => idtac
   end;
@@ -292,13 +300,13 @@ Definition ident_map := map_update (map_update (map_empty "nil") "_x" "x") "_y" 
 Definition precc_map := map_update (map_update (map_empty "nil") "x" "a") "y" "b".
 (*Map for postc.*)
 Definition postc_map := map_update (map_update (map_empty "nil") "x" "b") "y" "a".
-(*Algorithm:
+(*Algorithm: 
  1. Map : Precc. Map : Postc.
  2. Check: for every variable: if precc. maps to a ghost variable and not identifier -> read the variable into identifier
  3. Once all reading is done: Check that all precc. variables point to identifiers -> check for write
  4. Pre and Post same -> Exit
 *)
-Check (Sset (id_map (precc_map "x")) (Ederef (Etempvar (id_map (var_map "x")) (tptr tint)) tint)).
+Check (Sset (id_map (precc_map "x")) (Ederef (Etempvar (id_map (var_map "x")) (tptr tint)) tint)). 
 Check (Sset _a2 (Ederef (Etempvar _x (tptr tint)) tint)).
 
 Definition conc (s : string) := append (append "_" s) "2". (*used for variable names*)
@@ -309,55 +317,55 @@ Definition vars := ["x";"y"].
 Fixpoint updMap (varin : list string) (v1 v2 : string) (post_mcmap : total_map string) :=
   match varin with
   | nil => post_mcmap
-  | h :: t => if String.eqb (post_mcmap h) v1 then (updMap t v1 v2 (map_update post_mcmap h v2))
+  | h :: t => if String.eqb (post_mcmap h) v1 then (updMap t v1 v2 (map_update post_mcmap h v2)) 
               else (updMap t v1 v2 post_mcmap)
-  end.
+  end. 
 
 (*read: checks for a variable if read is applicable and does updates to the maps acco*)
-Definition read_identmap (x : string) :=
-  let v := (precc_map x) in (if (String.eqb (ident_map v) "nil") then
-  (let iden := conc v in
-   let idmp1 := map_update ident_map iden v in
-   let idpmp1 := map_update precc_map x iden in updMap vars v iden postc_map
-   )
+Definition read_identmap (x : string) := 
+  let v := (precc_map x) in (if (String.eqb (ident_map v) "nil") then 
+  (let iden := conc v in  
+   let idmp1 := map_update ident_map iden v in 
+   let idpmp1 := map_update precc_map x iden in updMap vars v iden postc_map  
+   )    
 else ident_map).
 
 
 (*required for read - first update is to identity map*)
-Definition upd_ident (idmap : total_map string) (x v : string) :=
+Definition upd_ident (idmap : total_map string) (x v : string) := 
   let iden := conc v in map_update idmap iden v.
 
 (*required for read - second update is to precc. map*)
-Definition upd_premap (pre_map : total_map string) (x iden : string) :=
+Definition upd_premap (pre_map : total_map string) (x iden : string) := 
   map_update pre_map x iden.
 
 (*required for read - third update is for postc. map*)
-Definition upd_postmap (post_map : total_map string) (v iden : string) :=
+Definition upd_postmap (post_map : total_map string) (v iden : string) := 
   updMap vars v iden post_map.
 
 
 (*write map: for a variable; check if its pre and postc. are both identifiers and both different identifiers
 map the pre id. to post*)
-Definition write_identmap (iden_map prec_map post_map : total_map string) (x : string) :=
-  let v1 := (prec_map x) in
-  let v2 := (post_map x) in
-  if (String.eqb (iden_map v1) "nil") then prec_map (*Read needs to happen*)
+Definition write_identmap (iden_map prec_map post_map : total_map string) (x : string) := 
+  let v1 := (prec_map x) in 
+  let v2 := (post_map x) in 
+  if (String.eqb (iden_map v1) "nil") then prec_map (*Read needs to happen*) 
   else if (String.eqb (iden_map v2) "nil") then prec_map  (*Read needs to happen*)
   else if (String.eqb v1 v2) then prec_map (*both are equal: frame*)
   else map_update prec_map x v2 (*update precc_map for x to point to v2*)
 .
 
-(* x -> a; y -> b | x -> b; y -> a     |  y -> _a2 |  y -> _a2*)
+(* x -> a; y -> b | x -> b; y -> a     |  y -> _a2 |  y -> _a2*) 
 Fixpoint readSynth (iden_map prec_map post_map : total_map string) (l : list string) :=
-  match l with
+  match l with 
   | nil => (iden_map, (prec_map, post_map))
-  | h :: t => let v := (prec_map h) in (if (String.eqb (iden_map v) "nil") then
-              (let iden := conc v in
-              let idmp := map_update iden_map iden v in
-              let idprmp := map_update prec_map h iden in
-              let idpomp := updMap vars v iden post_map in
-              readSynth idmp idprmp idpomp t
-              )
+  | h :: t => let v := (prec_map h) in (if (String.eqb (iden_map v) "nil") then 
+              (let iden := conc v in  
+              let idmp := map_update iden_map iden v in 
+              let idprmp := map_update prec_map h iden in 
+              let idpomp := updMap vars v iden post_map in 
+              readSynth idmp idprmp idpomp t  
+              )    
              else readSynth iden_map prec_map post_map t)
   end.
 
@@ -365,20 +373,20 @@ Fixpoint writeSynth (iden_map prec_map post_map : total_map string) (l : list st
   match l with
   | nil => prec_map (*only prec. map can change for write*)
   | h :: t => writeSynth iden_map (write_identmap iden_map prec_map post_map h) post_map t
-end.
+end. 
 
 Definition readRes := readSynth ident_map precc_map postc_map vars.
 
 
 Ltac matchReadLoc l a idG idT :=
-  match l with
+  match l with 
   | nil => eapply semax_seq' with (c1 := (Sset idG (Ederef (Etempvar idT (tptr tint)) tint)))
   | temp ?t a  :: ?l' => simpl
   | _ :: ?l' => matchReadLoc l' a idG idT
   end.
 
 Ltac matchReadSepAndTac s l v idG idT :=
-  match s with
+  match s with 
   | nil => simpl
   | data_at ?sh tint ?a v  :: ?t => (*match => call ltac loc*) matchReadLoc l a idG idT
   | _ :: ?t => matchReadSepAndTac t l v idG idT
@@ -392,53 +400,132 @@ Ltac readtac v idG idT  :=
 
 
 Ltac matchWriteLoc l a idV :=
-  match l with
-  | nil => simpl
+  match l with 
+  | nil => idtac a
   | temp ?t a  :: ?l' => eapply semax_seq' with (c1 := (Sassign (Ederef (Etempvar idV (tptr tint)) tint) (Etempvar t tint)))
   | _ :: ?l' => matchWriteLoc l' a idV
   end.
 
+(*determine if the placeholder is a constant or a variable*)
+Ltac detConstantOrVariable l a :=
+  match l with
+  | nil => false
+  | temp _ a :: _ => true
+  | _ :: ?t => detConstantOrVariable t a
+  end.
+
+(*fetch the identifier that is pointing to the variable*)
+(*temp _ _*)
+Ltac fetchVariable l a  :=
+  match l with
+  | nil => default
+  | temp ?t a :: ?l' => t
+  | _ :: ?l' => fetchVariable l' a
+  end.
+
+Print binary_operation.
+Ltac fetchOperator Op :=
+  match Op with
+  |Z.add _ _ => Oadd
+  |Z.sub _ _ => Osub
+  |Z.mul _ _ => Omul
+  |Z.eq_dec _ _ => Oeq
+  |Z_lt_ge_dec _ _ => Olt 
+  |Z_gt_le_dec _ _ => Ogt
+  |Z_le_gt_dec _ _ => Ole
+  |Z_ge_lt_dec _ _ => Oge
+  end.
+
 Ltac matchWriteSepAndTac s l v idV :=
   match s with
-  | nil => simpl
-  | data_at ?sh tint ?a v  :: ?t => matchWriteLoc l a idV
-  | _ :: ?t => matchWriteSepAndTac t l v idV
-  end.
+  | nil =>  fail
+  | data_at ?sh tint (Vint (Int.repr (?o' ?a' ?b'))) v  :: ?t => 
+      let ac := (detConstantOrVariable l (Vint (Int.repr a'))) in 
+      let bc := (detConstantOrVariable l (Vint (Int.repr b'))) in
+      let va := (fetchVariable l (Vint (Int.repr a'))) in 
+      let vb := (fetchVariable l (Vint (Int.repr b'))) in
+      let opbin := (fetchOperator (o' a' b')) in
+      match ac with
+      | true => match bc with
+                | true =>  eapply semax_seq' with (c1 := (Sassign (Ederef (Etempvar idV (tptr tint)) tint) (*both variables*)
+                          (Ebinop opbin (Etempvar va tint) (Etempvar vb tint) tint))) 
+                | false => eapply semax_seq' with (c1 := (Sassign (Ederef (Etempvar idV (tptr tint)) tint) (*a var, b const.*)
+                          (Ebinop opbin (Etempvar va tint) (Econst_int (Int.repr b') tint) tint)))
+                end 
+      | false => match bc with
+                 | true =>  eapply semax_seq' with (c1 := (Sassign (Ederef (Etempvar idV (tptr tint)) tint) (*a const. b var*)
+                          (Ebinop opbin (Econst_int (Int.repr a') tint) (Etempvar vb tint) tint)))
+                 | false => eapply semax_seq' with (c1 := (Sassign (Ederef (Etempvar idV (tptr tint)) tint) (*both const.*)
+                          (Ebinop opbin (Econst_int (Int.repr a') tint) (Econst_int (Int.repr b') tint) tint)))
+                 end 
+      end
+  | data_at ?sh tint (Vint (Int.repr ?a)) v  :: ?t => matchWriteLoc l (Vint (Int.repr a)) idV
+  | _ :: ?t =>  matchWriteSepAndTac t l v idV 
+  end. 
 
 (*x _x; x -> b; Check pre Loc. *)
 Ltac writetac v idV :=
-  match goal with
-  | |- semax _ (PROPx _ (LOCALx ?Lx (SEPx ?Sx))) _
+  match goal with 
+  | |- semax _ (PROPx _ (LOCALx ?Lx (SEPx ?Sx))) _ 
         (normal_ret_assert (PROPx _ (LOCALx _ (SEPx ?Spx)) * _)%logic) => matchWriteSepAndTac Spx Lx v idV
-  | |- semax _ (PROPx _ (LOCALx ?Lx (SEPx ?Sx))) _
+  | |- semax _ (PROPx _ (LOCALx ?Lx (SEPx ?Sx))) _ 
   (normal_ret_assert (fun rho : environ => ((PROPx _ (LOCALx _ (SEPx ?Spx))) rho * _ rho)%logic)) => matchWriteSepAndTac Spx Lx v idV
   end.
 
-Ltac foldtac :=
+Ltac ifAndTac l comp v1 v2 :=
+  let op := (fetchOperator (comp v1 v2)) in 
+  let ac := (fetchVariable l (Vint (Int.repr v1))) in 
+  let bc := (fetchVariable l (Vint (Int.repr v2))) in
+  apply semax_later_trivial; eapply semax_ifthenelse_PQR' with (b := (Ebinop op (Etempvar ac tint) (Etempvar bc tint) tint)).
+
+(*Ltac for if tactic*)
+Ltac conditional_writetac v idV b :=
   match goal with
-  | |- semax _ (PROPx _ (LOCALx ?Lx (SEPx ?Sx))) _
-          (normal_ret_assert ?N) => change (normal_ret_assert N) with abbreviate
+  | |- semax _ (PROPx _ (LOCALx ?Lx (SEPx ?Sx))) _  (normal_ret_assert (PROPx _ (LOCALx _ 
+              (SEPx (if ?comp ?a' ?b' then ?Spifx else ?Spex))) * _)%logic) => match b with
+                                                                               | true => matchWriteSepAndTac Spifx Lx v idV
+                                                                               | false => matchWriteSepAndTac Spex Lx v idV
+                                                                              end 
+  | |- semax _ (PROPx _ (LOCALx ?Lx (SEPx ?Sx))) _ (normal_ret_assert 
+               (fun rho : environ => ((PROPx _ (LOCALx _ 
+               (SEPx (if ?comp ?a' ?b' then ?Spifx else ?Spex)))) 
+               rho * _ rho)%logic)) => match b with
+                                       | true => matchWriteSepAndTac Spifx Lx v idV
+                                       | false => matchWriteSepAndTac Spex Lx v idV
+                                       end 
   end.
 
+(*Ltac for if tactic*)
+Ltac iftac :=
+  match goal with
+  | |- semax _ (PROPx _ (LOCALx ?Lx (SEPx ?Sx))) _  (normal_ret_assert (PROPx _ (LOCALx _ 
+              (SEPx (if ?comp ?a' ?b' then ?Spifx else ?Spex))) * _)%logic) => ifAndTac Lx comp a' b'
+  | |- semax _ (PROPx _ (LOCALx ?Lx (SEPx ?Sx))) _ (normal_ret_assert 
+               (fun rho : environ => ((PROPx _ (LOCALx _ (SEPx (if ?comp ?a' ?b' then ?Spifx else ?Spex)))) 
+                rho * _ rho)%logic)) => ifAndTac Lx comp a' b'
+  end.
+
+Definition swapnum (a b : Z) := (b, a).
+Check swapnum.
 
 Lemma body_swapsynthesisLtacs: exists s, semax_body Vprog Gprog (f_swap s)  swap_spec.
 Proof.
   eexists. start_functionaux.
+  unfold POSTCONDITION, abbreviate.
   readtac x _a2 _x. apply semax_later_trivial. load_tac. simpl.
-  (*readtac y _b2 _y.*)
+  (*readtac y _b2 _y.*) 
   readtac y _b2 _y. apply semax_later_trivial. load_tac. simpl.
   (*write - unfold*)
   unfold POSTCONDITION. unfold abbreviate.
   writetac y _y. apply semax_later_trivial. store_tac. simpl.
   (*second write*)
-  writetac x _x.
-  apply semax_later_trivial. store_tac. simpl.
+  writetac x _x. apply semax_later_trivial. store_tac. simpl.
   (*skip part*)
   unfold stackframe_of. simpl map. rewrite fold_right_nil. simpl.
   (*rewrite sepcon_emp.*)
   eapply semax_post. 5:{ eapply semax_skip. }
-  apply derives_ENTAIL. eapply drop_LOCAL'' with (n := O). eapply drop_LOCAL'' with (n := O).
-  eapply drop_LOCAL'' with (n := O). eapply drop_LOCAL'' with (n := O). simpl.
+  apply derives_ENTAIL. eapply drop_LOCAL'' with (n := O). eapply drop_LOCAL'' with (n := O). 
+  eapply drop_LOCAL'' with (n := O). eapply drop_LOCAL'' with (n := O). simpl. 
   intros. entailer!.
   apply derives_ENTAIL.
   simpl. intros. entailer!.
@@ -464,13 +551,12 @@ Proof.
   (*write*)
   Definition pre_writemap := writeSynth pread_idmap pre_rmap post_rmap vars.
   eapply semax_seq' with (c1 := (Sassign (Ederef (Etempvar (id_map (var_map "x")) (tptr tint)) tint) (Etempvar (id_map (pre_writemap "x")) tint))).
-  apply semax_later_trivial. store_tac. simpl.
+  apply semax_later_trivial. store_tac. simpl. 
   (*write second*)
   eapply semax_seq' with (c1 := (Sassign (Ederef (Etempvar (id_map (var_map "y")) (tptr tint)) tint) (Etempvar (id_map (pre_writemap "y")) tint)))(c2 := Sskip).
-  apply semax_later_trivial. store_tac. simpl.
+  apply semax_later_trivial. store_tac. simpl. 
   simpl. forward. entailer!.
 Qed.
-
 
 (*rules: Pre and Post -> decide*)
 (*swap synthesis*)
@@ -480,7 +566,7 @@ Proof.
   (*copy swap synthesis*)
   (*read*)
   eapply semax_seq' with (c1 := (Sset _a2 (Ederef (Etempvar _x (tptr tint)) tint))).
-  apply semax_later_trivial. load_tac. simpl.
+  apply semax_later_trivial. load_tac. simpl. 
   (*second read*)
   eapply semax_seq' with (c1 := (Sset _b2 (Ederef (Etempvar _y (tptr tint)) tint))).
   apply semax_later_trivial. load_tac. simpl.
@@ -506,17 +592,34 @@ Lemma body_swapmathsynthesis: exists s, semax_body Vprog Gprog (f_swapmath s)  s
 Proof.
   eexists. start_functionaux.
   (*read*)
-  eapply semax_seq' with (c1 := (Sset _a2 (Ederef (Etempvar _x (tptr tint)) tint))).
-  apply semax_later_trivial. load_tac. simpl.
-  (*second read*)
-  eapply semax_seq' with (c1 := (Sset _b2 (Ederef (Etempvar _y (tptr tint)) tint))).
-  apply semax_later_trivial. load_tac. simpl.
-  (*write*)
-  eapply semax_seq' with (c1 := (Sassign (Ederef (Etempvar _y (tptr tint)) tint)
-  (Ebinop Oadd (Etempvar _a2 tint) (Econst_int (Int.repr 1) tint) tint)))(c2 := Sskip).
-  apply semax_later_trivial. store_tac. simpl. forward. entailer!.
+  readtac x _a2 _x. apply semax_later_trivial. load_tac. simpl.
+  readtac y _b2 _y. apply semax_later_trivial. load_tac. simpl.
+  unfold POSTCONDITION, abbreviate.  
+  (*write - needs better ltac*)
+  writetac y _y. apply semax_later_trivial. store_tac. simpl.
+  (*skip*)
+  unfold stackframe_of. simpl map. rewrite fold_right_nil. simpl.
+  (*rewrite sepcon_emp.*)
+  eapply semax_post. 5:{ eapply semax_skip. }
+  apply derives_ENTAIL. eapply drop_LOCAL'' with (n := O). eapply drop_LOCAL'' with (n := O). 
+  eapply drop_LOCAL'' with (n := O). eapply drop_LOCAL'' with (n := O). simpl. 
+  intros. entailer!.
+  apply derives_ENTAIL.
+  simpl. intros. entailer!.
+  simpl. intros. entailer!. simpl. intros. entailer!.
 Qed.
 
+Lemma body_swapmathsynthesisWriteExp: exists s, semax_body Vprog Gprog (f_swapmath s)  swapmath_spec.
+Proof.
+  eexists. start_functionaux.
+  (*read*)
+  readtac x _a2 _x. apply semax_later_trivial. load_tac. simpl.
+  readtac y _b2 _y. apply semax_later_trivial. load_tac. simpl.
+  eapply semax_seq' with (c1 := (Sassign (Ederef (Etempvar _y (tptr tint)) tint)
+  (Ebinop Oadd (Etempvar _a2 tint) (Econst_int (Int.repr 1) tint) tint)))(c2 := Sskip).
+  apply semax_later_trivial. store_tac. forward. entailer!.
+  simpl. entailer!.
+Qed.
 
 
 Definition f_swapif (s : statement) := {|
@@ -553,3 +656,20 @@ Proof.
   apply semax_later_trivial. store_tac. simpl. forward.
   destruct (Z_lt_ge_dec a b) eqn:Hzlt. entailer!. entailer!.
 Qed.
+
+Lemma body_swapifsynthesisoth: exists s, semax_body Vprog Gprog (f_swapif s)  swapif_spec.
+Proof.
+  eexists. start_functionaux.
+  (*read a and b*)
+  readtac x _a2 _x. apply semax_later_trivial. load_tac. simpl.
+  readtac y _b2 _y. apply semax_later_trivial. load_tac. simpl.  
+  (*if-else*)
+  unfold POSTCONDITION, abbreviate. 
+  iftac. simpl. reflexivity. entailer!. entailer!.
+  conditional_writetac y _y true. apply semax_later_trivial. store_tac. simpl.
+  conditional_writetac x _x true. apply semax_later_trivial. store_tac. simpl.  
+Admitted.
+
+
+
+
