synthLemmas.v
@@ -1,0 +1,302 @@
+Require VC.Preface.  (* Check for the right version of VST *)
+Require Import VST.floyd.proofauto.
+Require Import VST.floyd.local2ptree_denote.
+Require Import VST.floyd.local2ptree_eval.
+Import compcert.lib.Maps.
+
+(*auxiliary start function 1: the function specific lemmas are commented out*)
+Ltac start_aux1 := 
+  (*leaf_function;*)
+  lazymatch goal with
+  | |- semax_body ?V ?G ?F ?spec =>
+      (*check_normalized F; function_body_unsupported_features F;*)
+         let s := fresh "spec" in
+          pose (s := spec); hnf in s; cbn zeta in s;
+           repeat
+            lazymatch goal with
+            | s:=(_, NDmk_funspec _ _ _ _ _):_ |- _ => fail
+            | s:=(_, mk_funspec _ _ _ _ _ _ _):_ |- _ => fail
+            | s:=(_, ?a _ _ _ _):_ |- _ => unfold a in s
+            | s:=(_, ?a _ _ _):_ |- _ => unfold a in s
+            | s:=(_, ?a _ _):_ |- _ => unfold a in s
+            | s:=(_, ?a _):_ |- _ => unfold a in s
+            | s:=(_, ?a):_ |- _ => unfold a in s
+            end;
+           lazymatch goal with
+           | s:=(_, WITH _ : globals PRE [ ] main_pre _ _ _ POST [tint] _):_
+             |- _ => idtac
+           | s:=?spec':_ |- _ => check_canonical_funspec spec'
+           end; change (semax_body V G F s); subst s; 
+           unfold NDmk_funspec'
+  end;
+  let DependedTypeList := fresh "DependedTypeList" in
+   unfold NDmk_funspec;
+    match goal with
+    | |- semax_body _ _ _ (_, mk_funspec _ _ _ ?Pre _ _ _) =>
+          split3; [ check_parameter_types' | check_return_type |  ];
+           match Pre with
+           | fun _ => convertPre _ _ (fun i => _) =>
+               intros Espec DependedTypeList i
+           | fun _ x => match _ with
+                        | (a, b) => _
+                        end =>
+               intros Espec DependedTypeList [a b]
+           | fun _ i => _ => intros Espec DependedTypeList i
+           end; simpl fn_body; simpl fn_params; simpl fn_return
+    end;
+    (*eliminates the rho environ part*)
+    try
+     match goal with
+     | |- semax _ (fun rho => (?A rho * ?B rho)%logic) _ _ =>
+           change (fun rho => (?A rho * ?B rho)%logic) with (A * B)%logic
+     end; 
+    simpl functors.MixVariantFunctor._functor in *;
+    simpl rmaps.dependent_type_functor_rec; clear DependedTypeList;
+    rewrite_old_main_pre;
+    repeat
+     match goal with
+     | |- semax _ (match ?p with
+                   | (a, b) => _
+                   end * _)%logic _ _ => destruct p as [a b]
+     | |-
+       semax _
+         (close_precondition _ match ?p with
+                               | (a, b) => _
+                               end * _)%logic _ _ => 
+       destruct p as [a b]
+     | |- semax _ (match ?p with
+                   | (a, b) => _
+                   end eq_refl * _)%logic _ _ => 
+       destruct p as [a b]
+     | |-
+       semax _
+         (close_precondition _ (match ?p with
+                                | (a, b) => _
+                                end eq_refl) * _)%logic _ _ =>
+           destruct p as [a b]
+     | |-
+       semax _
+         (close_precondition _
+            (fun ae =>
+             !! (Datatypes.length (snd ae) = ?A) &&
+             ?B (make_args ?C (snd ae) (mkEnviron (fst ae) _ _))) * _)%logic
+         _ _ =>
+           match B with
+           | match ?p with
+             | (a, b) => _
+             end => destruct p as [a b]
+           end
+     end; try start_func_convert_precondition.
+
+(*auxiliary start function2: This is exactly same as start_function2*)
+Ltac start_aux2 :=
+  first
+    [ erewrite compute_close_precondition_eq; [  | reflexivity | reflexivity ]
+    | rewrite close_precondition_main ].
+
+(*used in place of abbreviate_semax for start_aux3 to put POSTC. in apt. form*)
+Ltac abbreviate_semaxaux :=
+  match goal with
+  | |- semax _ FF _ _ => apply semax_ff
+  | |- semax _ (PROPx (False::_) _) _ _ => Intros; contradiction
+  | |- semax _ _ _ _ =>
+      simplify_Delta;
+      repeat match goal with
+      | MC := @abbreviate statement _ |- _ => unfold abbreviate in MC; subst MC
+      end;
+      (*force sequential is modified to support expansion*)
+      apply sequential; simpl_ret_assert;
+      match goal with |- semax _ _ _ ?Q =>
+          abbreviate Q : ret_assert as POSTCONDITION
+      end;
+      match goal with |- semax _ _ ?C _ =>
+        match C with
+        | Ssequence ?C1 ?C2 =>
+          (* use the next 3 lines instead of "abbreviate"
+          in case C1 contains an instance of C2 *)
+          let MC := fresh "MORE_COMMANDS" in
+          pose (MC := @abbreviate _ C2);
+          change C with (Ssequence C1 MC);
+          match C1 with
+          | Swhile _ ?C3 => abbreviate C3 as LOOP_BODY
+          | _ => idtac
+          end
+        | Swhile _ ?C3 => abbreviate C3 as LOOP_BODY
+        | _ => idtac
+        end
+        end
+  | |- _ |-- _ => unfold_abbrev_ret
+  end;
+  clear_abbrevs;
+  simpl typeof.
+
+
+Ltac start_aux3 :=
+  simpl app;
+  simplify_func_tycontext;
+  repeat match goal with
+  | |- context [Sloop (Ssequence (Sifthenelse ?e Sskip Sbreak) ?s) Sskip] =>
+       fold (Swhile e s)
+  | |- context [Ssequence ?s1 (Sloop (Ssequence (Sifthenelse ?e Sskip Sbreak) ?s2) ?s3) ] =>
+      match s3 with
+      | Sset ?i _ => match s1 with Sset ?i' _ => unify i i' | Sskip => idtac end
+      end;
+      fold (Sfor s1 e s2 s3)
+  end;
+  try expand_main_pre;
+  process_stackframe_of;
+  repeat change_mapsto_gvar_to_data_at;  (* should really restrict this to only in main,
+                                  but it needs to come after process_stackframe_of *)
+  repeat rewrite <- data_at__offset_zero;
+  try simple apply start_function_aux1; (*apply semax_extract_PROP.*)
+  repeat (apply semax_extract_PROP;
+              match goal with
+              | |- _ ?sh -> _ =>
+                 match type of sh with
+                 | share => intros ?SH
+                 | Share.t => intros ?SH
+                 | _ => intro
+                 end
+               | |- _ => intro
+               end);
+  abbreviate_semaxaux;
+  lazymatch goal with 
+  | |- semax ?Delta (PROPx _ (LOCALx ?L _)) _ _ => check_parameter_vals Delta L
+  | _ => idtac
+  end;
+  try match goal with DS := @abbreviate (PTree.t funspec) ?DS1 |- _ =>
+     unify DS1 (PTree.empty funspec); clearbody DS
+  end;
+  start_function_hint.
+
+(*start function*)
+Ltac start_functionaux := start_aux1; start_aux2; start_aux3.
+
+(*determine if read is possible - if so, then read*)
+Ltac matchReadLoc l a idG idT :=
+  match l with 
+  | nil => eapply semax_seq' with (c1 := (Sset idG (Ederef (Etempvar idT (tptr tint)) tint)))
+  | temp ?t a  :: ?l' => fail (*read fails, as pre and post are the same*)
+  | _ :: ?l' => matchReadLoc l' a idG idT
+  end.
+
+(*traverse the SEPx list and determine value of aå**)
+Ltac matchReadSepAndTac s l v idG idT :=
+  match s with 
+  | nil => simpl
+  | data_at ?sh tint ?a v  :: ?t => matchReadLoc l a idG idT
+  | _ :: ?t => matchReadSepAndTac t l v idG idT
+  end.
+
+(*read tactic - ltac; calls the ltacs above*)
+Ltac readtac v idG idT  :=
+  match goal with
+  | |- semax _ (PROPx _ (LOCALx ?Lx (SEPx ?Sx))) _ _ => matchReadSepAndTac Sx Lx v idG idT
+  end.
+
+(*apply write lemma if write is possible*)
+Ltac matchWriteLoc l a idV :=
+  match l with 
+  | nil => fail (*write not possible*)
+  | temp ?t a  :: ?l' => eapply semax_seq' with (c1 := (Sassign (Ederef (Etempvar idV (tptr tint)) tint) (Etempvar t tint)))
+  | _ :: ?l' => matchWriteLoc l' a idV
+  end.
+
+(*determine if the placeholder is a constant or a variable*)
+Ltac detConstantOrVariable l a :=
+  match l with
+  | nil => false
+  | temp _ a :: _ => true
+  | _ :: ?t => detConstantOrVariable t a
+  end.
+
+(*fetch the identifier that is pointing to the variable*)
+Ltac fetchVariable l a  :=
+  match l with
+  | nil => default
+  | temp ?t a :: ?l' => t
+  | _ :: ?l' => fetchVariable l' a
+  end.
+
+(*fetch the operator name: specific for operations involved in a op b*)
+Ltac fetchOperator Op :=
+  match Op with
+  |Z.add _ _ => Oadd
+  |Z.sub _ _ => Osub
+  |Z.mul _ _ => Omul
+  |Z.eq_dec _ _ => Oeq
+  |Z_lt_ge_dec _ _ => Olt 
+  |Z_gt_le_dec _ _ => Ogt
+  |Z_le_gt_dec _ _ => Ole
+  |Z_ge_lt_dec _ _ => Oge
+  end.
+
+(*different cases to consider for write*)
+Ltac matchWriteSepAndTac s l v idV :=
+  match s with
+  | nil =>  fail
+  | data_at ?sh tint (Vint (Int.repr (?o' ?a' ?b'))) v  :: ?t => 
+      let ac := (detConstantOrVariable l (Vint (Int.repr a'))) in 
+      let bc := (detConstantOrVariable l (Vint (Int.repr b'))) in
+      let va := (fetchVariable l (Vint (Int.repr a'))) in 
+      let vb := (fetchVariable l (Vint (Int.repr b'))) in
+      let opbin := (fetchOperator (o' a' b')) in
+      match ac with
+      | true => match bc with
+                | true =>  eapply semax_seq' with (c1 := (Sassign (Ederef (Etempvar idV (tptr tint)) tint) (*both variables*)
+                          (Ebinop opbin (Etempvar va tint) (Etempvar vb tint) tint))) 
+                | false => eapply semax_seq' with (c1 := (Sassign (Ederef (Etempvar idV (tptr tint)) tint) (*a var, b const.*)
+                          (Ebinop opbin (Etempvar va tint) (Econst_int (Int.repr b') tint) tint)))
+                end 
+      | false => match bc with
+                 | true =>  eapply semax_seq' with (c1 := (Sassign (Ederef (Etempvar idV (tptr tint)) tint) (*a const. b var*)
+                          (Ebinop opbin (Econst_int (Int.repr a') tint) (Etempvar vb tint) tint)))
+                 | false => eapply semax_seq' with (c1 := (Sassign (Ederef (Etempvar idV (tptr tint)) tint) (*both const.*)
+                          (Ebinop opbin (Econst_int (Int.repr a') tint) (Econst_int (Int.repr b') tint) tint)))
+                 end 
+      end
+  | data_at ?sh tint (Vint (Int.repr ?a)) v  :: ?t => matchWriteLoc l (Vint (Int.repr a)) idV
+  | _ :: ?t =>  matchWriteSepAndTac t l v idV 
+  end. 
+
+(*x _x; x -> b *)
+Ltac writetac v idV :=
+  match goal with 
+  | |- semax _ (PROPx _ (LOCALx ?Lx (SEPx ?Sx))) _ 
+        (normal_ret_assert (PROPx _ (LOCALx _ (SEPx ?Spx)) * _)%logic) => matchWriteSepAndTac Spx Lx v idV
+  | |- semax _ (PROPx _ (LOCALx ?Lx (SEPx ?Sx))) _ 
+  (normal_ret_assert (fun rho : environ => ((PROPx _ (LOCALx _ (SEPx ?Spx))) rho * _ rho)%logic)) => matchWriteSepAndTac Spx Lx v idV
+  end.
+
+Ltac ifAndTac l comp v1 v2 :=
+  let op := (fetchOperator (comp v1 v2)) in 
+  let ac := (fetchVariable l (Vint (Int.repr v1))) in 
+  let bc := (fetchVariable l (Vint (Int.repr v2))) in
+  apply semax_later_trivial; eapply semax_ifthenelse_PQR' with (b := (Ebinop op (Etempvar ac tint) (Etempvar bc tint) tint)).
+
+(*Ltac for if tactic*)
+Ltac conditional_writetac v idV b :=
+  match goal with
+  | |- semax _ (PROPx _ (LOCALx ?Lx (SEPx ?Sx))) _  (normal_ret_assert (PROPx _ (LOCALx _ 
+              (SEPx (if ?comp ?a' ?b' then ?Spifx else ?Spex))) * _)%logic) => match b with
+                                                                               | true => matchWriteSepAndTac Spifx Lx v idV
+                                                                               | false => matchWriteSepAndTac Spex Lx v idV
+                                                                              end 
+  | |- semax _ (PROPx _ (LOCALx ?Lx (SEPx ?Sx))) _ (normal_ret_assert 
+               (fun rho : environ => ((PROPx _ (LOCALx _ 
+               (SEPx (if ?comp ?a' ?b' then ?Spifx else ?Spex)))) 
+               rho * _ rho)%logic)) => match b with
+                                       | true => matchWriteSepAndTac Spifx Lx v idV
+                                       | false => matchWriteSepAndTac Spex Lx v idV
+                                       end 
+  end.
+
+(*Ltac for if tactic*)
+Ltac iftac :=
+  match goal with
+  | |- semax _ (PROPx _ (LOCALx ?Lx (SEPx ?Sx))) _  (normal_ret_assert (PROPx _ (LOCALx _ 
+              (SEPx (if ?comp ?a' ?b' then ?Spifx else ?Spex))) * _)%logic) => ifAndTac Lx comp a' b'
+  | |- semax _ (PROPx _ (LOCALx ?Lx (SEPx ?Sx))) _ (normal_ret_assert 
+               (fun rho : environ => ((PROPx _ (LOCALx _ (SEPx (if ?comp ?a' ?b' then ?Spifx else ?Spex)))) 
+                rho * _ rho)%logic)) => ifAndTac Lx comp a' b'
+  end.
